LeanLTL/Examples/TeaserITP2025.lean
@@ -6,8 +6,7 @@ open scoped LeanLTL.Notation
 noncomputable section
 namespace Teaser
 axiom σ : Type*
-axiom p : σ → ℤ
-abbrev n : TraceFun σ ℤ := TraceFun.of p
+axiom n : σ → ℤ
 
 example : ⊨ⁱ LLTL[((← n) = 5 ∧ G ((X (← n)) = (← n) ^ 2)) → G (5 ≤ (← n))] := by
   rw [TraceSet.sem_entail_inf_iff]
